

1.3 a) $X(t) = e^{-q|t|}$, $q > 0$

Separieren $t \geq 0$ y $t < 0$:

$$X(\omega) = \int_0^{\infty} e^{-qt} e^{-j\omega t} dt + \int_{-\infty}^0 e^{qt} e^{-j\omega t} dt$$

$$\int_0^{\infty} e^{-(q+j\omega)t} dt = \frac{1}{q+j\omega} \cdot \int_0^{\infty} e^{-t} dt$$

$$\int_{-\infty}^0 e^{(q-j\omega)t} dt = \frac{1}{q-j\omega}$$

$$X(\omega) = \frac{1}{q+j\omega} + \frac{1}{q-j\omega} = \frac{2q}{q^2 + \omega^2}$$

b) $x(t) = \cos(\omega_c t)$

$$\cos(\omega_c t) = \frac{1}{2} (e^{j\omega_c t} + e^{-j\omega_c t})$$

$$X(\omega) = \frac{1}{2} (2\pi\delta(\omega - \omega_c) + 2\pi\delta(\omega + \omega_c))$$

$$= \pi [\delta(\omega - \omega_c) + \delta(\omega + \omega_c)]$$

c) $x(t) = \sin(\omega_s t)$

$$\sin(\omega_s t) = \frac{1}{2j} (e^{j\omega_s t} - e^{-j\omega_s t})$$

$$X(\omega) = \frac{1}{2j} (2\pi\delta(\omega - \omega_s) - 2\pi\delta(\omega + \omega_s)) = \frac{\pi}{j} [\delta(\omega - \omega_s) - \delta(\omega + \omega_s)]$$

$$d) x(t) = f(t) \cos(\omega_c t)$$

$$f(t) \cos(\omega_c t) = \frac{1}{2} f(t) e^{j\omega_c t} + \frac{1}{2} f(t) e^{-j\omega_c t}$$

$$X(\omega) = \frac{1}{2} F(\omega - \omega_c) + \frac{1}{2} F(\omega + \omega_c)$$

$$e) x(t) = e^{-at^2}, \quad a > 0$$

$$X(\omega) = \int_{-\infty}^{\infty} e^{-at^2} e^{-j\omega t} dt = \sqrt{\frac{\pi}{a}} e^{-\frac{\omega^2}{4a}}$$

$$f) x(t) = A \text{rect}_d(t) \rightarrow X(\omega) = A \int_{-d/2}^{d/2} e^{-j\omega t} dt = A \left[\frac{e^{-j\omega t}}{-j\omega} \right]_{-d/2}^{d/2} = \frac{A(e^{-j\omega d/2} - e^{j\omega d/2})}{-j\omega}$$

$$X(\omega) = A \frac{\sin(\omega d/2)}{\omega} = Ad \frac{\sin(\omega d/2)}{\omega d/2}$$

$$= Ad \text{sinc}\left(\frac{\omega d}{2}\right)$$

$$\bullet \text{sinc}(x) = \frac{\sin x}{x}$$

$$1.4) a. \mathcal{F}\{e^{-j\omega_1 t} \cos(\omega_c t)\}$$

$$\mathcal{F}\{e^{j\omega_0 t} x(t)\} = X(\omega - \omega_0)$$

$$\mathcal{F}\{\cos(\omega_c t)\} = \pi [\delta(\omega - \omega_c) + \delta(\omega + \omega_c)]$$

$$e^{-j\omega_1 t} = e^{j(-\omega_1)t} \rightarrow \omega_0 = -\omega_1$$

$$\mathcal{F}\{e^{-j\omega_1 t} \cos(\omega_c t)\} = \pi [\delta(\omega + \omega_1 - \omega_c) + \delta(\omega + \omega_1 + \omega_c)]$$

$$b. \mathcal{F}\{u(t) \cos^2(\omega_c t)\} \quad (u(t) = \text{escalón unitario})$$

$$\rightarrow \cos^2(\omega_c t) = \frac{1}{2} + \frac{1}{2} \cos(2\omega_c t)$$

$$u(t) \cos^2(\omega_c t) = \frac{1}{2} u(t) + \frac{1}{2} u(t) \cos(2\omega_c t)$$

$$\mathcal{F}\{u(t)\} = \pi \delta(\omega) + \frac{1}{j\omega}$$

$$\rightarrow \mathcal{F}\{u(t) e^{j\omega_0 t}\} = \pi \delta(\omega - \omega_0) + \frac{1}{j(\omega - \omega_0)}$$

$$\rightarrow \cos(2\omega_c t) = \frac{1}{2} (e^{j2\omega_c t} + e^{-j2\omega_c t})$$

$$\mathcal{F}\{u(t) \cos^2(\omega_c t)\} = \frac{1}{2} \left(\pi \delta(\omega) + \frac{1}{j\omega} \right)$$

$$+ \frac{1}{4} \left(\pi \delta(\omega - 2\omega_c) + \frac{1}{j(\omega - 2\omega_c)} \right) + \frac{1}{4} \left(\pi \delta(\omega + 2\omega_c) + \frac{1}{j(\omega + 2\omega_c)} \right)$$

$$c) \mathcal{F}^{-1} \left\{ \frac{7}{(w^2 + 6w + 45)} \cdot \frac{7}{(8 + jw)^2} \right\}$$

$$x(t) = \mathcal{F}^{-1} \{ A(w) B(w) \} = \frac{7}{2\pi} a(t) \cdot b(t)$$

$$\rightarrow a(t) = \mathcal{F}^{-1} \{ A(w) \}, \quad b(t) = \mathcal{F}^{-1} \{ B(w) \}$$

• Primer factor:

$$w^2 + 6w + 45 = (w + 3)^2 + 36$$

$$\mathcal{F} \{ e^{-q|t|} e^{jw_0 t} \} = \frac{2q}{q^2 + (w - w_0)^2} \quad \rightarrow q=6 \quad w_0=-3$$

$$\mathcal{F} \{ e^{-6|t|} e^{j3t} \} = \frac{12}{(w+3)^2 + 36}$$

$$\mathcal{F}^{-1} \left\{ \frac{7}{(w^2 + 6w + 45)} \right\} = \frac{7}{12} e^{-6|t|} e^{j3t}$$

• Segundo factor

$$\frac{7}{(8 + jw)^2} \quad q > 0$$

$$\mathcal{F} \{ t e^{-qt} u(t) \} = \frac{7}{(q + jw)^2}$$

$$\mathcal{F}^{-1} \left\{ \frac{7}{(8 + jw)^2} \right\} = t e^{-8t} u(t)$$

$$x(t) = \frac{7}{2\pi} \left(\frac{7}{12} e^{-6|t|} e^{j3t} \right) \cdot (t e^{-8t} u(t))$$

$$d) \mathcal{F}\{3t^2\}$$

$$\mathcal{F}\{t^n x(t)\} = j^n \frac{d^n}{d\omega^n} X(\omega)$$

$$\rightarrow \mathcal{F}\{t^n\} = 2\pi j^n \delta^{(n)}(\omega)$$

$$n=2: \rightarrow \mathcal{F}\{t^2\} = 2\pi j^2 \delta''(\omega) = -2\pi \delta''(\omega)$$

$$\mathcal{F}\{3t^2\} = -6\pi \delta''(\omega)$$

$$e) \frac{B}{T} \sum_{n=-\infty}^{\infty} \left(\frac{1}{a^2 + (\omega - n\omega_0)^2} + \frac{1}{a + j(\omega - n\omega_0)} \right)$$

inversa de $\frac{1}{a^2 + (\omega - \omega_0)^2}$

$$\text{Usando } \mathcal{F}\{e^{-a|t|} e^{j\omega_0 t}\} = \frac{2a}{a^2 + (\omega - \omega_0)^2}$$

despejamos:

$$\mathcal{F}^{-1}\left\{\frac{1}{a^2 + (\omega - n\omega_0)^2}\right\} = \frac{1}{2a} e^{-a|t|} e^{jn\omega_0 t}$$

$$\sum_n \frac{1}{a^2 + (\omega - n\omega_0)^2} \rightarrow \frac{1}{2a} e^{-a|t|} \sum_n e^{jn\omega_0 t}$$

$$\mathcal{F}^{-1}\left\{\sum_n \frac{1}{a^2 + (\omega - n\omega_0)^2}\right\} = \frac{1}{2a} \cdot \frac{2\pi}{\omega_0} \sum_k e^{-a|kT|} \delta(t - kT)$$

$$= \frac{\pi}{a\omega_0} \sum_k e^{-a|kT|} \delta(t - kT)$$

$$\omega_0 = 2\pi/T \rightarrow \frac{T}{2a} \sum_k e^{-a|kT|} \delta(t - kT)$$

• Inversa de $\frac{1}{a + j(\omega - n\omega_0)}$

$$\rightarrow F\{u(t) e^{-at} e^{jn\omega_0 t}\} = \frac{1}{a + j(\omega - n\omega_0)}$$

$$\sum_n \frac{1}{a + j(\omega - n\omega_0)} \rightarrow u(t) e^{-at} \sum_n e^{jn\omega_0 t}$$

$$F^{-1}\left\{\sum_n \frac{1}{a + j(\omega - n\omega_0)}\right\} = \frac{2\pi}{\omega_0} \sum_k u(kT) e^{-a kT} \delta(t - kT)$$

Con $\omega_0 = 2\pi/T$

$$\frac{2\pi}{\omega_0} \sum_{k=0}^{\infty} e^{-a kT} \delta(t - kT) \rightarrow T \sum_{k=0}^{\infty} e^{-a kT} \delta(t - kT)$$

$$\boxed{\frac{B}{2a} \sum_{k=-\infty}^{\infty} e^{-a|kT|} \delta(t - kT) + B \sum_{k=0}^{\infty} e^{-a kT} \delta(t - kT)}$$